

In this document, we formally prove the following Theorem:

Theorem 1. *If $\Gamma \vdash p$ then p is NI_t^Γ .*

In Section 1, we present *semantics rules* and the *typing rules* of the language. In Section 2, we present the definitions and lemmas used to prove the theorem. In Section 3, we prove the Lemmas and Theorem 1.

1 Semantics and Type Rules

1.1 Semantic Rules

$$\begin{array}{c}
\text{BASE} \\
\frac{}{\mu \vdash v \Rightarrow v}
\end{array}
\quad
\begin{array}{c}
\text{VAR} \\
\frac{\Gamma(x) = v}{\mu \vdash x \Rightarrow v}
\end{array}
\quad
\begin{array}{c}
\text{OP} \\
\frac{\mu \vdash e \Rightarrow v, \mu \vdash e' \Rightarrow v'}{\mu \vdash e \circ e' \Rightarrow \square \vee v \vee v'}
\end{array}$$

$$\begin{array}{c}
\text{UPDATE} \\
\frac{\mu \vdash e \Rightarrow v, m \in \text{dom}(\mu)}{\mu \vdash m := e \Rightarrow \square \mu[m := v]}
\end{array}
\quad
\begin{array}{c}
\text{SEQUENCE} \\
\frac{\mu \vdash c \Rightarrow^{t'} \mu', \mu' \vdash c' \Rightarrow^{t''} \mu''}{\mu \vdash c; c' \Rightarrow^{t'.t''} \mu''}
\end{array}$$

$$\begin{array}{c}
\text{BRANCH-TRUE} \\
\frac{\mu \vdash e \Rightarrow \text{true}, \mu \vdash c \Rightarrow^t \mu'}{\mu \vdash \text{if } e \text{ then } c \text{ else } c' \Rightarrow^t \mu'}
\end{array}
\quad
\begin{array}{c}
\text{BRANCH-FALSE} \\
\frac{\mu \vdash e \Rightarrow \text{false}, \mu \vdash c \Rightarrow^t \mu'}{\mu \vdash \text{if } e \text{ then } c \text{ else } c' \Rightarrow^t \mu'}
\end{array}$$

$$\begin{array}{c}
\text{LOOP-TRUE} \\
\frac{\mu \vdash e \Rightarrow \text{true}, \quad \mu \vdash c \Rightarrow^t \mu', \quad \mu' \vdash \text{while } e \text{ do } c \Rightarrow^{t'} \mu''}{\mu \vdash \text{while } e \text{ do } c \Rightarrow^{t.t'} \mu''}
\end{array}
\quad
\begin{array}{c}
\text{LOOP-FALSE} \\
\frac{\mu \vdash e \Rightarrow \text{false}}{\mu \vdash \text{while } e \text{ do } c \Rightarrow \square \mu}
\end{array}$$

$$\begin{array}{c}
\text{SECURE BROADCAST} \\
\frac{vk = KG(\{"n_1", "n_2", \dots, "n_n"\}, v') \quad \mu \vdash K \Rightarrow v' \quad \mu \vdash e \Rightarrow "m" \quad \mu(L) = \{"n_1", "n_2", \dots, "n_n"\} \quad \mu \vdash pc \Rightarrow v}{\mu \vdash \text{sbroadcast}(L, e || pc, K) \Rightarrow^{\text{BEnc}(L, vk, "m" || "v")} \mu}
\end{array}$$

$$\begin{array}{c}
\text{ENDORSE-RA} \\
\frac{\mu(L) = \{"n_0", "n_1", \dots, "n_n"\} \quad \mu(L') = \{"n'_0", "n'_1", \dots, "n'_n"\} \quad \mu \vdash \text{Ra}(L) \Rightarrow S \quad S \subseteq \{"n_0", \dots, "n_n"\}}{\mu \vdash \text{for } n \in L \text{ endorse Ra}(L, L', n) \Rightarrow \mu'[L := L \setminus S; L' := L' \cup S]}
\end{array}$$

1.2 Type Rules

LIT $\Gamma \vdash n : \tau$	VAR $\frac{\Gamma(x) = \tau \text{ var}}{\Gamma \vdash x : \tau \text{ var}}$	LVAR $\frac{\Gamma(L) = \tau \text{ Lvar}}{\Gamma \vdash L : \tau \text{ Lvar}}$	KVAR $\frac{\Gamma(K) = \top \text{ Kvar}}{\Gamma \vdash K : \top \text{ Kvar}}$
OP $\frac{\Gamma \vdash e : \tau \quad \Gamma \vdash e' : \tau}{\Gamma \vdash e \circ e' : \tau}$	ASSIGN $\frac{\Gamma \vdash x : \tau \text{ var} \quad \Gamma \vdash e' : \tau}{\Gamma \vdash x := e' : \tau \text{ cmd}}$	ASSIGN-COUNTER $\frac{\Gamma \vdash \text{pc} : \perp \text{ Cvar}}{\Gamma \vdash \text{pc} := \text{pc} + 1 : \perp \text{ cmd}}$	SEQUENCE $\frac{\Gamma \vdash c : \tau \text{ cmd} \quad \Gamma \vdash c' : \tau \text{ cmd}}{\Gamma \vdash c; c' : \tau \text{ cmd}}$
IF $\frac{\Gamma \vdash e : \tau \quad \Gamma \vdash c : \tau \text{ cmd} \quad \Gamma \vdash c' : \tau \text{ cmd}}{\Gamma \vdash \text{if } e \text{ then } c \text{ else } c' : \tau \text{ cmd}}$	WHILE $\frac{\Gamma \vdash e : \tau \quad \Gamma \vdash c : \tau \text{ cmd}}{\Gamma \vdash \text{while } e \text{ do } c : \tau \text{ cmd}}$	SBROADCAST $\frac{\Gamma \vdash e' : \tau \quad \Gamma \vdash L : \tau \text{ Lvar} \quad \Gamma \vdash K : \top \text{ Kvar} \quad \Gamma \vdash \text{pc} : \perp \text{ Cvar}}{\Gamma \vdash \text{sbroadcast}(L, e' \text{pc}, K) : \tau \text{ cmd}}$	REMOTE ATTESTATION $\frac{\Gamma \vdash L : \tau \text{ Lvar} \quad \Gamma \vdash L' : \tau' \text{ Lvar} \quad I(\tau') \leq_I I(\tau) \quad C(\tau) \leq_C C(\tau')}{\Gamma \vdash \text{for } n \in L \text{ endorse Ra}(L, L', n) : \tau \text{ cmd}}$

Subtyping rules

BASE $\frac{\tau \leq \tau'}{\vdash \tau \subseteq \tau'}$	S-VAR $\frac{\Gamma \vdash x : \tau \text{ var}}{\Gamma \vdash x : \tau}$	S-CVAR $\frac{\Gamma \vdash \text{pc} : \perp \text{ Cvar}}{\Gamma \vdash \text{pc} : \perp}$
CMD $\frac{\vdash \tau \subseteq \tau'}{\vdash \tau' \text{ cmd} \subseteq \tau \text{ cmd}}$	SUBTYPE $\frac{\Gamma \vdash p : \rho \quad \vdash \rho \subseteq \rho'}{\Gamma \vdash p : \rho'}$	

2 Definitions and Lemmas

Definition 1 (τ – Equal Memories). *Two memories μ_0, μ_1 are τ – Equal for Γ , written $\mu_0 =_{\tau}^{\Gamma} \mu_1$, iff $\text{dom}(\mu_0) = \text{dom}(\mu_1) \wedge \forall x \in \mu_0$ such that if $\Gamma(x) = \tau' \text{ var} \wedge \tau' \leq \tau$, then $\mu_0(x) = \mu_1(x)$.*

Definition 2 (Filtering). *Let $\text{filter}_{\tau}(t) = \text{filter}'_{\tau}(t, [])$ and $\text{filter}'_{\tau}([], t) = t$.*

$$\text{filter}'_{\tau}(\text{BEnc}(L, \text{vk}, v' || v) \cdot t', t) = \begin{cases} \text{filter}'_{\tau}(t', t \cdot (L, v')) & \text{if } \Gamma(L) \leq \tau \\ \text{filter}'_{\tau}(t', t) & \text{Otherwise} \end{cases}$$

Definition 3 (NonInterference). *A server program p is NI at τ for Γ , written $NI_{\tau}^{\Gamma}(p)$, iff $\forall \mu_0, \mu_1$ such that $\mu_0 =_{\tau}^{\Gamma} \mu_1 \wedge \mu_0 \vdash p \Rightarrow^{t_0} \mu'_0 \wedge \mu_1 \vdash p \Rightarrow^{t_1} \mu'_1$, then $\mu'_0 =_{\tau}^{\Gamma} \mu'_1 \wedge \text{filter}(t_0) = \text{filter}(t_1)$.*

Lemma 1. (*LowExpression*) $\forall \tau, \tau', \mu_0, \mu_1$, if $\mu_0 =_{\tau}^{\Gamma} \mu_1$ and $\Gamma \vdash e : \tau'$ and $\tau' \leq \tau$ and $\mu_0 \vdash e \Rightarrow v_0$ and $\mu_1 \vdash e \Rightarrow v_1$, then $v_0 = v_1$.

Lemma 2. (*HighCommand*) $\forall \tau, \tau', \mu, \mu', t$, if $\Gamma \vdash c : \tau'$ cmd and $\tau' \not\leq \tau$ and $\mu \vdash c \Rightarrow^t \mu'$, then $\mu =_{\tau}^{\Gamma} \mu'$ and $\text{filter}_{\tau}(t) = []$.

3 Proof

3.1 Proof of Lemma 1

Proof. We prove Lemma 1 by structural induction on e with $P_{Struct}(e) = n$. According to our type system, specifically the subtyping rule $S\text{-}Var$, only variables of type τ *var* can be typed as τ . That is the reason we omit the cases of $NVar$ and $MKVar$.

It follows that:

- $P_{Struct}(v) = 1$.
- $P_{Struct}(x) = 1$.
- $P_{Struct}(e \circ e') = P_{Struct}(e) + P_{Struct}(e')$.

From the hypothesis of Lemma 1, we have that:

$$(H_1) \mu_0 \stackrel{\Gamma}{=}_{\tau} \mu_1.$$

$$(H_2) \Gamma \vdash e : \tau'.$$

$$(H_3) \tau' \leq \tau.$$

$$(H_4) \mu_0 \vdash e \Rightarrow v_0.$$

$$(H_5) \mu_1 \vdash e \Rightarrow v_1.$$

And we need to prove that:

$$(G_1) v_0 = v_1.$$

Case 1 (Base Case).

Subcase 1.1 (Lit: v). By (H_2) and the typing rule *Lit*, we have that:

$$(H_6) \Gamma \vdash v : \tau'.$$

By (H_4) and the semantics rule *Base*, we have that:

$$(H_7) \mu_0 \vdash v \Rightarrow v.$$

By (H_5) and the semantics rule *Base*, we have that:

$$(H_8) \mu_1 \vdash v \Rightarrow v.$$

From (H_7) and (H_8) , (G_1) is trivially true.

Subcase 1.2 (Var: x). By (H_2) and the subtyping rule $S\text{-}Var$ (which is the only rule that allows variables of type τ' *var* to be typed as variables of type τ'), we have that:

$$(H_6) \Gamma \vdash x : \tau' \text{ var}.$$

By (H_6) and the typing rule *Var*, we have that:

$$(H_7) \quad \Gamma(x) = \tau' \text{ var.}$$

By (H_4) and the semantics rule *Var*, we have that:

$$(H_8) \quad \mu_0(x) = v_0.$$

By (H_5) and the semantics rule *Var*, we have that:

$$(H_9) \quad \mu_1(x) = v_1.$$

By Definition 1 and (H_1) of Lemma 1, we have that:

$$\forall y, \mu_0(y) = \mu_1(y), \text{ if } \Gamma(y) = \tau' \text{ var} \wedge \tau' \leq \tau$$

From this, and by (H_6) and (H_3) , we have that :

$$(H_{10}) \quad \mu_0(x) = \mu_1(x).$$

By (H_{10}) , (H_8) and (H_9) , we conclude that $v_0 = v_1$, which is (G_1) .

Case 2 (*Op*: $e' \circ e''$). **Inductive hypothesis for e**

For $P_{Struct}(e) = n$, we have that:

$$(IH_1) \quad \mu_0 =_{\tau}^{\Gamma} \mu_1.$$

$$(IH_2) \quad \Gamma \vdash e : \tau'.$$

$$(IH_3) \quad \tau' \leq \tau.$$

$$(IH_4) \quad \mu_0 \vdash e \Rightarrow v_0.$$

$$(IH_5) \quad \mu_1 \vdash e \Rightarrow v_1.$$

Then we conclude that:

$$(IH_6) \quad v_0 = v_1.$$

Inductive case: height = $P_{Struct}(e) = n + 1$.

Op: $e' \circ e''$. For the typing rule *Op*, we have that:

$$(H_1) \quad \Gamma \vdash e' : \tau'.$$

$$(H_2) \quad \Gamma \vdash e'' : \tau'.$$

By (IH_4) and the semantics rule *Op*, we have that:

$$(H_3) \quad \mu_0 \vdash e' \Rightarrow v_0.$$

$$(H_4) \quad \mu_0 \vdash e'' \Rightarrow v'_0.$$

$$(H_5) \mu_0 \vdash e' \circ e'' \Rightarrow v_0 \circ v'_0.$$

By (IH₅) and the semantics rule Op, we have that:

$$(H_6) \mu_1 \vdash e' \Rightarrow v_1.$$

$$(H_7) \mu_1 \vdash e'' \Rightarrow v'_1.$$

$$(H_8) \mu_1 \vdash e' \circ e'' \Rightarrow v_1 \circ v'_1.$$

Concerning e' , from the inductive hypothesis on e , it follows that:

$$(H_6) v_0 = v_1.$$

Concerning e'' , from the inductive hypothesis on e , it follows that:

$$(H_7) v'_0 = v'_1.$$

By the transitive property of $=$ and since $v_0 = v_1$ and $v'_0 = v'_1$, we conclude that $v_0 \cdot v'_0 = v_1 \cdot v'_1$, which is (G₁).

□

To prove Theorem ??, we rely on Lemma ?? and ?. Since Lemma ?? is analogous to the one in Appendix ??, we only prove Lemma ?? and Theorem ??.

3.2 Proof of Lemma ??

Proof. We prove this lemma by structural induction on c with $P_{Struct}(c) = n$. It follows that:

- $P_{Struct}(x := e') = 1$.
- $P_{Struct}(pc := pc + 1) = 1$.
- $P_{Struct}(sbroadcast(L, e || pc, K)) = 1$.
- $P_{Struct}(\text{for } n \in L \text{ Ra}(L, L', n)) = 1$.
- $P_{Struct}(c'; c'') = P_{Struct}(c') + P_{Struct}(c'')$.
- $P_{Struct}(\text{while } e \text{ do } c) = P_{Struct}(c) + 1$.
- $P_{Struct}(\text{if } e \text{ then } c' \text{ else } c'' = \text{MAX}(P_{Struct}(c'), P_{Struct}(c'')) + 1$.

From the hypothesis of Lemma ??, we have that:

$$(H_1) \quad \Gamma \vdash c : \tau' \text{ cmd.}$$

$$(H_2) \quad \tau' \not\leq \tau.$$

$$(H_3) \quad \mu \vdash c \Rightarrow^t \mu'.$$

And we need to prove that:

$$(G_1) \quad \mu \stackrel{\Gamma}{=}_{\tau} \mu'.$$

$$(G_2) \quad \text{filter}_{\tau}(t) = [].$$

Case 1 (Base case).

Subcase 1.1 (Assign: $x := e'$). By the hypothesis of the lemma, we have that:

$$(H_4) \quad \Gamma \vdash x := e' : \tau' \text{ cmd.}$$

By (H_4) and the typing rule Assign, we have that:

$$(H_5) \quad \Gamma \vdash x : \tau' \text{ var.}$$

$$(H_6) \quad \Gamma \vdash e : \tau'.$$

By (H_5) and the typing rule Var, we have that:

$$(H_7) \quad \Gamma(x) = \tau' \text{ var.}$$

By (H_3) and the semantics rule Update, we have that:

(H₈) $\mu \vdash e \Rightarrow v$.

(H₉) $\mu' \vdash x := e \Rightarrow^t \mu[x := v]$.

By the semantics rule *Update*, we have that:

(H₁₀) $t = []$.

For (H₂), we have that $\tau' \not\leq \tau$. Since the only variable in which μ and μ' are different is x by (H₉) and the security level of the variable x is $\tau' \text{var}$, we can conclude that $\mu =_{\tau}^{\Gamma} \mu'$ which is (G₁).

To prove (G₂), by (H₁₀), $t = []$. Therefore $\text{filter}_{\tau}(t) = []$.

Subcase 1.2 (Assign-Counter: $\text{pc} := \text{pc} + 1$). By the hypothesis of the lemma, we have that:

(H₄) $\Gamma \vdash \text{pc} := \text{pc} + 1 : \perp \text{cmd}$.

By (H₄) and the typing rule *Assign-Counter*, we have that:

(H₅) $\Gamma \vdash \text{pc} : \perp \text{Cvar}$.

By (H₃) and the semantics rule *Update*, we have that:

(H₆) $\mu \vdash \text{pc} + 1 \Rightarrow v$.

(H₇) $\mu' \vdash \text{pc} := \text{pc} + 1 \Rightarrow^t \mu[\text{pc} := v]$.

By the semantics rule *Update*, we have that:

(H₈) $t = []$.

For (H₂), we have that $\tau' \not\leq \tau$. Since the only variable in which μ and μ' are different is pc by (H₇) and the security level of the variable pc is $\perp' \text{Cvar}$, we can conclude that $\mu =_{\tau}^{\Gamma} \mu'$ which is (G₁).

To prove (G₂), by (H₈), $t = []$. Therefore $\text{filter}_{\tau}(t) = []$.

Subcase 1.3 (SBroadcast: $\text{sbroadcast}(L, e \parallel \text{pc}, K)$). By the hypothesis of the lemma, we have that:

(H₄) $\Gamma \vdash \text{sbroadcast}(L, e \parallel \text{pc}, K) : \tau' \text{cmd}$.

By (H₄) and the typing rule *SBroadcast*, we have that:

(H₅) $\Gamma \vdash e : \tau'$.

(H₆) $\Gamma \vdash L : \tau' \text{Lvar}$.

(H₇) $\Gamma \vdash K : \top \text{Kvar}$.

(H₈) $\Gamma \vdash \text{pc} : \perp \text{Cvar}$.

By (H₃) and the semantics rule *Secure Broadcast*, we have that:

$$(H_9) \mu \vdash \text{sbroadcast}(L, e \parallel \text{pc}, K) \Rightarrow^t \mu.$$

By the semantics rule *Secure Broadcast*, we have that:

$$(H_{10}) t = \text{BEnc}(L, \text{vk}, \text{"m"} \parallel \text{"v"}).$$

For (H₂), we have that $\tau' \not\leq \tau$. Since the initial memory μ and the final memory μ are equal by (H₉), we conclude that $\mu \stackrel{\Gamma}{=} \mu'$ which is (G₁).

To prove (G₂), by (H₁₀), $t = \text{BEnc}(L, \text{vk}, \text{"m"} \parallel \text{"v"})$. By Definition 2, and by (H₂) and (H₆), $\Gamma(L) \not\leq \tau$, therefore $\text{filter}_\tau(t) = []$.

Subcase 1.4 (Remote Attestation: for $n \in L \text{ Ra}(L, L', n)$). By the hypothesis of the lemma, we have that:

$$(H_4) \Gamma \vdash \text{for } n \in L \text{ Ra}(L, L', n) : \tau' \text{ cmd.}$$

By (H₄) and the typing rule *Remote Attestation*, we have that:

$$(H_5) \Gamma \vdash L : \tau' \text{ Lvar.}$$

$$(H_6) \Gamma \vdash L' : \tau'' \text{ Lvar.}$$

$$(H_7) \Gamma \vdash K : \top \text{ Kvar.}$$

$$(H_8) \Gamma \vdash \text{pc} : \perp \text{ Cvar.}$$

$$(H_9) I(\tau'') \leq_I I(\tau').$$

$$(H_{10}) C(\tau' \leq_C C(\tau'')).$$

By (H₃) and the semantics rule *Endorse-Ra*, we have that:

$$(H_{11}) \mu \vdash \text{for } n \in L \text{ Ra}(L, L', n) \Rightarrow^t \mu[L := L \setminus S; L' := L' \cup S].$$

By the semantics rule *Endorse-Ra*, we have that:

$$(H_{12}) t = [].$$

For (H₂), we have that $\tau' \not\leq \tau$. By (H₉) and (H₁₀) we have that $\tau' \leq \tau''$, therefore $\tau'' \not\leq \tau$. Since $\tau' \not\leq \tau$ and $\tau'' \not\leq \tau$ and because μ and μ' are different only for variables L of type τ' and L' of type τ'' by (H₉), we conclude that $\mu \stackrel{\Gamma}{=} \mu'$ which is (G₁).

To prove (G₂), by (H₁₀), $t = []$. Therefore $\text{filter}_\tau(t) = []$.

Inductive hypothesis for c For $P_{\text{Struct}}(c) = n$, we have that:

$$(IH_1) \Gamma \vdash c : \tau' \text{ cmd.}$$

$$(IH_2) \mu \vdash c \Rightarrow^t \mu'.$$

$$(IH_3) \tau' \not\leq \tau.$$

Then we conclude that:

$$(IH_4) \mu \stackrel{\Gamma}{=} \mu'.$$

$$(IH_5) \text{filter}_\tau(t) = [].$$

Inductive case: height $= P_{Struct}(c) = n + 1$.

Sequence: $c'; c''$. For the typing rule *Sequence*, we have that:

$$(H_1) \quad \Gamma \vdash c' : \tau' \text{ cmd.}$$

$$(H_2) \quad \Gamma \vdash c'' : \tau' \text{ cmd.}$$

By (IH_2) and the semantics rule *Sequence*, we have that:

$$(H_3) \quad \mu \vdash c' \Rightarrow^{t'} \mu'.$$

$$(H_4) \quad \mu' \vdash c'' \Rightarrow^{t''} \mu''.$$

$$(H_5) \quad \mu \vdash c'; c'' \Rightarrow^{t' \cdot t''} \mu''.$$

Concerning c' , from the inductive hypothesis on c , it follows that:

$$(H_6) \quad \mu =_{\tau}^{\Gamma} \mu'.$$

$$(H_7) \quad \text{filter}_{\tau}(t') = [].$$

Concerning c'' , from the inductive hypothesis on c , it follows that:

$$(H_8) \quad \mu' =_{\tau}^{\Gamma} \mu''.$$

$$(H_9) \quad \text{filter}_{\tau}(t'') = [].$$

By the transitive property of $=_{\tau}^{\Gamma}$ and since $\mu =_{\tau}^{\Gamma} \mu'$ and $\mu' =_{\tau}^{\Gamma} \mu''$, we can conclude $\mu =_{\tau}^{\Gamma} \mu''$.

In the semantics rule *Sequence*, $t' \cdot t''$ denotes the concatenation of two traces t' and t'' . Since $\text{filter}_{\tau}(t') = []$ by (H_7) and $\text{filter}_{\tau}(t'') = []$ by (H_9) , we conclude that $\text{filter}_{\tau}(t' \cdot t'') = []$.

While: while e do c . For the typing rule *While*, we have that:

$$(H_1) \quad \Gamma \vdash c : \tau' \text{ cmd.}$$

$$(H_2) \quad \Gamma \vdash e : \tau'.$$

By (H_1) and because the height of $\Gamma \vdash \text{while } e \text{ do } c$ is $n + 1$, we know that the height of the typing derivation tree of (H_1) is $\leq n$. By applying the inductive hypothesis on c , we get that:

$$(H_3) \quad \mu =_{\tau}^{\Gamma} \mu'.$$

$$(H_4) \quad \text{filter}_{\tau}(t) = [].$$

We want to prove that the inductive hypothesis works for while e do c also. By the hypothesis of Lemma ??, we have that if:

$(H'_0) \Gamma \vdash \text{while } e \text{ do } c : \tau' \text{ cmd.}$

$(H'_1) \mu \vdash \text{while } e \text{ do } c \Rightarrow^{t \cdot t'} \mu''.$

$(H'_2) \tau' \not\leq \tau.$

Then we want to prove that:

$(G_1) \mu =_{\tau}^{\Gamma} \mu''.$

$(G_2) \text{filter}_{\tau}(t \cdot t') = [].$

By the semantics rule of Loop, we have that:

$(H'_3) \mu \vdash e \Rightarrow v.$

$(H'_4) \mu \vdash c \Rightarrow^t \mu'.$

$(H'_5) \mu' \vdash \text{while } e \text{ do } c \Rightarrow^{t'} \mu''.$

Base case. *The only possibility for the semantics tree to be of height = 2 is when $v = \text{False}$.*

$$\frac{\mu \vdash e \Rightarrow \text{False}}{\mu \vdash \text{while } e \text{ do } c \Rightarrow^{[]} \mu}$$

By (H'_3) we conclude that $\mu =_{\tau}^{\Gamma} \mu$. We also conclude that $\text{filter}_{\tau}([]) = []$.

Assuming that our inductive hypothesis holds for the case of while when evaluating the height of the semantics tree $\leq m$, we want to prove the case of While with height $= m + 1$.

$$\frac{\mu \vdash e \Rightarrow \text{True} \quad (1) \mu \vdash c \Rightarrow^t \mu'' \quad (H'_6) \mu'' \vdash \text{while } e \text{ do } c' \Rightarrow^{t'} \mu'}{\mu \vdash \text{while } e \text{ do } c' \Rightarrow^{t \cdot t'} \mu'}$$

By applying the structural induction to (1), we have that $\mu =_{\tau}^{\Gamma} \mu''$ and $\text{filter}_{\tau}(t) = []$. By applying the inductive hypothesis on while e do c by (H'_6) , we can conclude that $\mu'' =_{\tau}^{\Gamma} \mu'$ and $\text{filter}_{\tau}(t') = []$. By applying the transitive property on $=_{\tau}^{\Gamma}$, we can conclude that $\mu'' =_{\tau}^{\Gamma} \mu'$ which is (G_1) . Moreover, since $\text{filter}_{\tau}(t) = []$ and $\text{filter}_{\tau}(t') = []$, and $t \cdot t'$ is a concatenation, then $\text{filter}_{\tau}(t \cdot t') = []$ which is (G_2) .

If: if e then c' else c'' . *For the typing rule If, we have that:*

$(H_1) \Gamma \vdash c' : \tau' \text{ cmd.}$

$(H_2) \Gamma \vdash c'' : \tau' \text{ cmd.}$

$(H_3) \Gamma \vdash e : \tau.$

By (H_1) and the inductive hypothesis on c' , we get that:

$$(H_4) \mu \stackrel{\Gamma}{=}_{\tau} \mu'.$$

$$(H_5) \text{filter}_{\tau}(t) = [].$$

By (H_1) and the inductive hypothesis on c'' , we get that:

$$(H_6) \mu \stackrel{\Gamma}{=}_{\tau} \mu'.$$

$$(H_7) \text{filter}_{\tau}(t') = [].$$

Concerning if e then c' else c'' , by the hypothesis of Lemma ??, we have that if:

$$(H_8) \Gamma \vdash \text{if } e \text{ then } c' \text{ else } c'' : \tau' \text{ cmd.}$$

$$(H_9) \mu \vdash \text{if } e \text{ then } c' \text{ else } c'' \Rightarrow^t \mu'.$$

$$(H_{10}) \mu \vdash \text{if } e \text{ then } c' \text{ else } c'' \Rightarrow^t \mu'.$$

$$(H_{11}) \tau' \not\leq \tau.$$

Then we want to prove that:

$$(G_1) \mu \stackrel{\Gamma}{=}_{\tau} \mu'.$$

$$(G_2) \text{filter}_{\tau}(t) = [].$$

By the semantics rule of Branch- True, we have that:

$$(H_{12}) \mu \vdash e \Rightarrow v.$$

$$(H_{13}) \mu \vdash c' \Rightarrow^t \mu'.$$

$$(H_{14}) t = [].$$

By (H_3) and (H_4) we can conclude that $\mu \stackrel{\Gamma}{=}_{\tau} \mu'$. By (H_5) and (H_{14}) we conclude that $\text{filter}_{\tau}(t) = []$.

By the semantics rule of Branch- False, we have that:

$$(H_{15}) \mu \vdash e \Rightarrow v.$$

$$(H_{16}) \mu \vdash c'' \Rightarrow^t \mu'.$$

$$(H_{17}) t = [].$$

By (H_3) and (H_5) we can conclude that $\mu \stackrel{\Gamma}{=}_{\tau} \mu'$. By (H_6) and (H_{17}) we conclude that $\text{filter}_{\tau}(t) = []$.

□

3.3 Proof of Theorem ??

Proof. By Definition ??, for p to be NI_{τ}^{Γ} , we need to prove that:

$$(G_1) \mu'_0 =_{\tau}^{\Gamma} \mu'_1.$$

$$(G_2) \text{filter}_{\tau}(t_0) = \text{filter}_{\tau}(t_1).$$

We prove this theorem by induction on the height of typing derivation tree $\Gamma \vdash p$.

Case 1. *Base case: height = 2*

Subcase 1.1. $p \triangleq x := e'$.

Concerning (G_1) and (G_2) , by Definition ??, we have that:

$$(H_1) \mu_0 =_{\tau}^{\Gamma} \mu_1.$$

$$(H_2) \mu_i \vdash x := e' \Rightarrow^{t_i} \mu'_i.$$

Moreover, for the semantics rule Update we have that:

$$(H_3) t_i = [].$$

Hence, by the semantics rule Update and (H_2) , we have that:

$$(H_4) \mu_i \vdash e' \Rightarrow v_i.$$

$$(H_5) \mu'_i = \mu_i[x := v_i].$$

By the hypothesis of Theorem ??, we have:

$$(H_6) \Gamma \vdash x := e' : \tau' \text{ cmd}.$$

By (H_6) and the typing rule Assign, we have that:

$$(H_7) \Gamma \vdash x : \tau' \text{ var}.$$

$$(H_8) \Gamma \vdash e' : \tau'.$$

By (H_7) and the typing rule Var, we have:

$$(H_9) \Gamma(x) = \tau' \text{ var}.$$

Depending on τ' , we have two cases:

$$(H_{10}) \tau' \leq \tau.$$

By Lemma ?? that can be applied due to (H_1) , (H_8) , (H_{10}) and (H_4) then

$$(H_{11}) : v_0 = v_1.$$

To prove (G_1) , we rely on the Definition ?? that states that $\mu_0 =_{\tau}^{\Gamma} \mu_1$, if $\forall x \in \mu_0$ such that $\Gamma(x) = \tau' \text{ var}$ and $\tau' \leq \tau$ then $\mu_0(x) = \mu_1(x)$.

Since (H_1) holds and the only variable in which μ_i and μ'_i are different is x by (H_5) , then we need to prove that $\mu_0(x) = \mu_1(x)$ which holds by (H_{11}) .

To prove (G_2) we rely on the Definition 2 and (H_3) . Since $t_0 = t_1 = []$ then $\text{filter}_{\tau}(t_0) = \text{filter}_{\tau}(t_1)$.

Since we proved (G_1) and (G_2) , then p is NI_{τ}^{Γ} .

(H₁₂) $\tau' \not\leq \tau$.

To prove (G₁), we rely on the Definition ?? that states that $\mu_0 =_{\tau}^{\Gamma} \mu_1$, if $\forall y \in \mu_0$ such that $\Gamma(y) = \tau'$ var and $\tau' \leq \tau$ then $\mu_0(y) = \mu_1(y)$. For (H₁₂), we have that $\tau' \not\leq \tau$. Since we are only interested by variables with security level less or equal than τ , we can conclude by (H₅) and (H₁) that $\mu'_0 =_{\tau}^{\Gamma} \mu'_1$.

To prove (G₂) we rely on the Definition 2 and (H₃). Since $t_0 = t_1 = []$ then $\text{filter}_{\tau}(t_0) = \text{filter}_{\tau}(t_1)$.

Since we proved (G₁) and (G₂), then p is NI_{τ}^{Γ} .

Subcase 1.2. $p \triangleq \text{pc} := \text{pc} + 1$.

Concerning (G₁) and (G₂), by Definition ??, we have that:

(H₁) $\mu_0 =_{\tau}^{\Gamma} \mu_1$.

(H₂) $\mu_i \vdash \text{pc} := \text{pc} + 1 \Rightarrow^{\tau_i} \mu'_i$.

By the semantics rule Update we have that:

(H₃) $t_i = []$.

Moreover, by the semantics rule Update and (H₂), we have that:

(H₄) $\mu_i \vdash \text{pc} + 1 \Rightarrow v_i$.

(H₅) $\mu'_i = \mu_i[x := v_i]$.

By the hypothesis of Theorem ??, we have:

(H₆) $\Gamma \vdash \text{pc} := \text{pc} + 1 : \perp \text{cmd}$.

By the typing rule Assign-Counter, we have that:

(H₇) $\Gamma \vdash \text{pc} : \perp \text{Cvar}$.

To prove (G₁), we rely on the Definition ?? that states that $\mu_0 =_{\tau}^{\Gamma} \mu_1$, if $\forall y \in \mu_0$ such that $\Gamma(y) = \tau'$ var and $\tau' \leq \tau$ then $\mu_0(y) = \mu_1(y)$. For (H₇), $\Gamma(\text{pc}) = \perp \text{Cvar}$. Since we are only interested in variables of type τ' var, we conclude by (H₅) and (H₁) that $\mu'_0 =_{\tau}^{\Gamma} \mu'_1$.

To prove (G₂) we rely on the Definition 2 and (H₃). Since $t_0 = t_1 = []$ then $\text{filter}_{\tau}(t_0) = \text{filter}_{\tau}(t_1)$.

Since we proved (G₁) and (G₂), then p is NI_{τ}^{Γ} .

Subcase 1.3. $p \triangleq \text{sbroadcast}(L, e || \text{pc}, K)$.

Concerning (G₁) and (G₂), by Definition ??, we have that:

(H₁) $\mu_0 =_{\tau}^{\Gamma} \mu_1$.

(H₂) $\mu_i \vdash \text{sbroadcast}(L, e || \text{pc}, K) \Rightarrow^{\tau_i} \mu_i$.

By the semantics rule Secure Broadcast, we have:

(H₃) $t_i = \text{BEnc}(L, vk_i, "m" || "v")$.

(H₄) $\mu_i \vdash K \Rightarrow v'_i$.

(H₅) $\mu_i \vdash e \Rightarrow "m_i"$.

(H₆) $\mu_i \vdash pc \Rightarrow v_i$.

(H₇) $\mu_i(L) = \{"n_0", "n_1", \dots, "n_n"\}$.

By the hypothesis of Theorem ??, we have:

(H₈) $\Gamma \vdash \text{sbroadcast}(L, e || pc, K) : \tau' \text{ cmd}$.

By (H₈) and the typing rule SBroadcast, we have:

(H₉) $\Gamma \vdash e : \tau'$.

(H₁₀) $\Gamma \vdash L : \tau' \text{ Lvar}$.

(H₁₁) $\Gamma \vdash K : \top \text{ Kvar}$.

(H₁₂) $\Gamma \vdash pc : \perp \text{ Cvar}$.

To prove (G₁), we rely on the Definition ?? that states that $\mu_0 =_{\tau}^{\Gamma} \mu_1$, if $\forall y \in \mu_0$ such that $\Gamma(y) = \tau' \text{ var}$ and $\tau' \leq \tau$ then $\mu_0(y) = \mu_1(y)$. For (H₉ – H₁₂), all the variables types are different than $\tau' \text{ var}$. Since we are only interested in variables of type $\tau' \text{ var}$, (G₁) follows by (H₁) and (H₂).

To prove (G₂), we have two cases:

(H₁₃) $\Gamma(L) \leq \tau'$

Being $\mu'_0 =_{\tau}^{\Gamma} \mu'_1$ and by (H₂) and (H₃) we have that $t_0 = t_1$. For an execution that starts with μ_0 , $t_0 = \text{BEnc}(L, vk_0, "m" || "v")$ and for an execution that starts with μ_1 , $t_1 = \text{BEnc}(L, vk_1, "m" || "v")$. By (H₁₃), $\Gamma(L) \leq \tau'$ then $\text{filter}_{\tau}(t_0) = [L, m]$ and $\text{filter}_{\tau}(t_1) = [L, m]$. It results that $\text{filter}_{\tau}(t_0) = \text{filter}_{\tau}(t_1)$ and therefore we prove (G₂).

Since we proved (G₁) and (G₂), then p is NI_{τ}^{Γ} .

(H₁₄) $\Gamma(L) \not\leq \tau'$

Being $\mu'_0 =_{\tau}^{\Gamma} \mu'_1$ and by (H₂) and (H₃) we have that $t_0 = t_1$. For an execution that starts with μ_0 , $t_0 = \text{BEnc}(L, vk_0, "m" || "v")$ and for an execution that starts with μ_1 , $t_1 = \text{BEnc}(L, vk_1, "m" || "v")$. By (H₁₄), $\Gamma(L) \not\leq \tau'$, then $\text{filter}_{\tau}(t_0) = []$ and $\text{filter}_{\tau}(t_1) = []$. It results that $\text{filter}_{\tau}(t_0) = \text{filter}_{\tau}(t_1)$ and therefore we prove (G₂).

Since we proved (G₁) and (G₂), then p is NI_{τ}^{Γ} .

Subcase 1.4. $p \stackrel{\Delta}{=} \text{for } n \in L \text{ endorse Ra}(L, L', n)$.

Concerning (G₁) and (G₂), by Definition ??, we have that:

(H₁) $\mu_0 =_{\tau}^{\Gamma} \mu_1$.

(H₂) $\mu_i \vdash \text{for } n \in L \text{ endorse } \text{Ra}(L, L', n) \Rightarrow^{t_i} \mu'_i$.

By the semantics rule *Endorse-Ra* we have that:

(H₃) $t_i = []$.

(H₄) $\mu_i \vdash \text{Ra}(L) \Rightarrow S$.

(H₅) $\mu_i(L) = \{ "n_0", "n_1", \dots, "n_n" \}$.

(H₆) $\mu_i(L') = \{ "n'_0", "n'_1", \dots, "n'_n" \}$.

By (H₂) and the semantics rule *Endorse-Ra* we have that:

(H₇) $\mu'_i = \mu_i[L := L \setminus S; L' := L' \cup S]$.

By the hypothesis of Theorem ??, we have:

(H₈) $\Gamma \vdash \text{for } n \in L \text{ endorse } \text{Ra}(L, L', n) : \tau' \text{ cmd}$.

By (H₈) and the typing rule *Remote Attestation*, we have that:

(H₉) $\Gamma \vdash L : \tau' \text{ Lvar}$.

(H₁₀) $\Gamma \vdash L' : \tau'' \text{ Lvar}$.

(H₁₁) $\Gamma \vdash K : \top \text{ Kvar}$.

(H₁₂) $\Gamma \vdash \text{pc} : \perp \text{ Cvar}$.

To prove (G₁), we rely on the Definition ?? that states that $\mu_0 \stackrel{\Gamma}{=} \mu_1$, if $\forall y \in \mu_0$ such that $\Gamma(y) = \tau' \text{ var}$ and $\tau' \leq \tau$ then $\mu_0(y) = \mu_1(y)$. For (H₉ – H₁₂), all the variables types are different than $\tau' \text{ var}$. Since we are only interested in variables of type $\tau' \text{ var}$, (G₁) follows by (H₁) and (H₂).

To prove (G₂) we rely on the Definition 2 and (H₃). Since $t_0 = t_1 = []$ then $\text{filter}_{\tau}(t_0) = \text{filter}_{\tau}(t_1)$.

Since we proved (G₁) and (G₂), then p is NI_{τ}^{Γ} .

Case 2 (Case: height $\leq n$). We will state our inductive hypothesis for a program c :

For the hypothesis of the theorem, we have that:

(IH₁) $\Gamma \vdash c : \tau' \text{ cmd}$.

(IH₂) $\mu_0 \stackrel{\Gamma}{=} \mu_1$.

For the derivation tree of height $\leq n$, we have that:

(IH₃) $\mu_0 \vdash c \Rightarrow^{t_0} \mu'_0$.

(IH₄) $\mu_1 \vdash c \Rightarrow^{t_1} \mu'_1$.

Then we conclude that:

(IH₅) $\mu'_0 \stackrel{\Gamma}{=} \mu'_1$.

(IH₆) $\text{filter}_\tau(t_0) = \text{filter}_\tau(t_1)$.

We suppose that (IH₁ – IH₆) are valid for programs of height $\leq n$ of typing derivation tree $\Gamma \vdash p$.

Case 3. Inductive case: height = $n + 1$

Subcase 3.1. $p \triangleq c'; c''$.

We want to prove that $\Gamma \vdash c'; c''$ is NI_τ^Γ . We assume that c' and c'' are of height $\leq n$, and $c'; c''$ of height $n + 1$.

For the typing rule Sequence, we have that:

(H₁) $\Gamma \vdash c' : \tau' \text{ cmd.}$

(H₂) $\Gamma \vdash c'' : \tau' \text{ cmd.}$

For the semantics rule Sequence, we have that:

(H₃) $\mu_i \vdash c' \Rightarrow^{t'_i} \mu'_i$.

(H₄) $\mu'_i \vdash c'' \Rightarrow^{t''_i} \mu''_i$.

Concerning c' , from the inductive hypotheses, it follows that:

(H₅) $\mu_{c'_0} \stackrel{\Gamma}{=} \mu_{c'_1}$.

(H₆) $\mu_{c'_0} \vdash c \Rightarrow^{t'_0} \mu'_{c'_0}$

(H₇) $\mu_{c'_1} \vdash c \Rightarrow^{t'_1} \mu'_{c'_1}$

(H₈) $\mu'_{c'_0} \stackrel{\Gamma}{=} \mu'_{c'_1}$.

(H₉) $\text{filter}_\tau(t'_0) = \text{filter}_\tau(t'_1)$.

It follows that c' is NI_τ^Γ .

Concerning c'' , from the inductive hypotheses, it follows that:

(H₁₀) $\mu_{c''_0} \stackrel{\Gamma}{=} \mu_{c''_1}$.

(H₁₁) $\mu_{c''_0} \vdash c \Rightarrow^{t''_0} \mu'_{c''_0}$

(H₁₂) $\mu_{c''_1} \vdash c \Rightarrow^{t''_1} \mu'_{c''_1}$

(H₁₃) $\mu'_{c''_0} \stackrel{\Gamma}{=} \mu'_{c''_1}$.

(H₁₄) $\text{filter}_\tau(t''_0) = \text{filter}_\tau(t''_1)$.

It follows that c'' is NI_{τ}^{Γ} .

In the semantics rule *Sequence*, we use $t' \cdot t''$ to denote the concatenation of two traces t' and t'' . By (H_9) and (H_{14}) we have that $t'_0 = t'_1$ and $t''_0 = t''_1$, which implies that $t'_0 \cdot t''_0 = t'_1 \cdot t''_1$. We conclude that $\text{filter}_{\tau}(t'_0 \cdot t''_0) = \text{filter}_{\tau}(t'_1 \cdot t''_1)$.

Since c' , c'' are NI_{τ}^{Γ} and $\text{filter}_{\tau}(t'_0 \cdot t''_0) = \text{filter}_{\tau}(t'_1 \cdot t''_1)$, we conclude that $\Gamma \vdash c'; c''$ is NI_{τ}^{Γ} .

Subcase 3.2. $p \triangleq \text{while } e \text{ do } c$.

For the typing rule *While*, we have that:

$(H_1) \quad \Gamma \vdash c : \tau' \text{ cmd.}$

$(H_2) \quad \Gamma \vdash e : \tau'.$

In the following, we show by induction that c is NI_{τ}^{Γ} .

By (H_1) and because the height of $\Gamma \vdash \text{while } e \text{ do } c$ is $n + 1$, we know that the height of the typing derivation tree of (H_1) is $\leq n$. Hence, we can apply the inductive hypothesis and get:

$(H_3) \quad \mu_0 =_{\tau}^{\Gamma} \mu_1.$

$(H_4) \quad \mu_0 \vdash c \Rightarrow^{t_0} \mu'_0.$

$(H_5) \quad \mu_1 \vdash c' \Rightarrow^{t_1} \mu'_1.$

Then,

$(H_6) \quad \mu'_0 =_{\tau}^{\Gamma} \mu'_1.$

$(H_7) \quad \text{filter}_{\tau}(t_0) = \text{filter}_{\tau}(t_1).$

We want to prove that $\text{while } e \text{ do } c$ is NI_{τ}^{Γ} . By the hypothesis of the theorem, we have that if:

$(H'_0) \quad \Gamma \vdash \text{while } e \text{ do } c : \tau' \text{ cmd.}$

$(H'_1) \quad \mu_0 =_{\tau}^{\Gamma} \mu_1.$

$(H'_2) \quad \mu_0 \vdash \text{while } e \text{ do } c \Rightarrow^{t_0} \mu'_0.$

$(H'_3) \quad \mu_1 \vdash \text{while } e \text{ do } c \Rightarrow^{t_1} \mu'_1.$

Then, we want to prove that:

$(G_0) \quad \mu'_0 =_{\tau}^{\Gamma} \mu'_1.$

$(G_1) \quad \text{filter}_{\tau}(t_0) = \text{filter}_{\tau}(t_1).$

By (H'_2) and the semantics rule of *Loop*, we have that:

$(H'_4) \quad \mu_0 \vdash e \Rightarrow v_0.$

By (H'_3) and the semantics rule of Loop, we have that:

$$(H'_5) \mu_1 \vdash e \Rightarrow v_1.$$

Depending on τ' , we have two cases:

Subcase 3.2.1. $\Gamma \vdash e : \tau', \tau' \leq \tau$.

$$(H'_6) \tau' \leq \tau.$$

In the case of (H'_6) , we check if we can apply the Subtype rule on While command. We would like to check if the command While of type τ' cmd can be typable as τ'' cmd, where $\tau'' \not\leq \tau'$. If the Subtype rule can be applied, the the proof of this case is analogous to Subcase 3.2.2.

Otherwise, if the Subtype rule cannot be applied, then by Lemma ?? that can be applied on (H'_1) , (H_2) , (H'_6) , (H'_4) and (H'_5) , we conclude that $v_0 = v_1$.

We prove this case by induction on the height of the semantics tree of (H'_2) . (We do not show this formally, but we rely on the fact that the height of (H'_2) is equal to the height of (H'_3) by Lemma ??).

Base case: height = 2. The only possibility for the semantics tree to be of height = 2 is:

- $v_0 = v_1 = \text{False}$.

$$\frac{\mu_0 \vdash e \Rightarrow \text{False}}{\mu_0 \vdash \text{while } e \text{ do } c \Rightarrow^{t_0} \mu_0}$$

$$\frac{\mu_1 \vdash e \Rightarrow \text{False}}{\mu_1 \vdash \text{while } e \text{ do } c \Rightarrow^{t_1} \mu_1}$$

We have that $\mu'_0 =_{\tau}^{\Gamma} \mu_0$ and $\mu'_1 =_{\tau}^{\Gamma} \mu_1$. We conclude by (H'_1) that $\mu'_0 =_{\tau}^{\Gamma} \mu'_1$. Moreover, since $t_0 = t_1 = []$ then $\text{filter}_{\tau}(t_0) = \text{filter}_{\tau}(t_1)$.

Assuming that our inductive hypothesis holds for the case of While when evaluating the height of semantics tree $\leq m$ with $\Gamma \vdash e : \tau', \tau' \leq \tau$, let us prove the case of While with height = $m + 1$.

Inductive case: height = $m + 1$.

$$\frac{\mu_0 \vdash e \Rightarrow \text{True} \quad \mu_0 \vdash c \Rightarrow^{t_0} \mu''_0 \quad (H'_7) \mu''_0 \vdash \text{while } e \text{ do } c \Rightarrow^{t'_0} \mu'_0}{\mu_0 \vdash \text{while } e \text{ do } c \Rightarrow^{t_0 \cdot t'_0} \mu'_0}$$

The height of (H'_2) is $m + 1$.

$$\frac{\mu_1 \vdash e \Rightarrow \text{True} \quad \mu_1 \vdash c \Rightarrow^{t_1} \mu''_1 \quad (H'_8) \mu''_1 \vdash \text{while } e \text{ do } c \Rightarrow^{t'_1} \mu'_1}{\mu_1 \vdash \text{while } e \text{ do } c \Rightarrow^{t_1 \cdot t'_1} \mu'_1}$$

The height of (H'_3) is $m + 1$.

By the previous induction on c , we have that $\mu'_0 =^\Gamma_\tau \mu'_1$ and $\text{filter}_\tau(t_0) = \text{filter}_\tau(t_1)$, through $\mu_0 =^\Gamma_\tau \mu_1$, $\mu_0 \vdash c' \Rightarrow^{t_0} \mu'_0$ and $\mu_1 \vdash c' \Rightarrow^{t_1} \mu'_1$.

Moreover, by induction on $\text{while } e \text{ do } c$ by (H'_7) and (H'_8) , we can conclude that $\mu'_0 =^\Gamma_\tau \mu'_1$ which is already our goal (G_1) and $\text{filter}_\tau(t'_0) = \text{filter}_\tau(t'_1)$. This is because we have that $\mu'_0 =^\Gamma_\tau \mu'_1$ and $\mu'_0 \vdash \text{while } e \text{ do } c \Rightarrow^{t'_0} \mu'_0$ and $\mu'_1 \vdash \text{while } e \text{ do } c \Rightarrow^{t'_1} \mu'_1$.

Since $t_i \cdot t'_i$ is the concatenation of two traces t_i and t'_i , and since $\text{filter}_\tau(t_0) = \text{filter}_\tau(t_1)$ and $\text{filter}_\tau(t'_0) = \text{filter}_\tau(t'_1)$, we conclude that $\text{filter}_\tau(t_0 \cdot t'_0) = \text{filter}_\tau(t_1 \cdot t'_1)$ from which (G_2) follows.

Since (G_1) and (G_2) are satisfied, then $\text{while } e \text{ do } c$ is NI^Γ_τ .

Subcase 3.2.2. $\Gamma \vdash e : \tau', \tau' \not\leq \tau$.

$(H'_9) \tau' \not\leq \tau$.

By Lemma ?? that can be applied on (H_1) , (H_4) , (H_5) and (H'_9) , we conclude that $\mu_i =^\Gamma_\tau \mu'_i$.

We prove that $\mu'_0 =^\Gamma_\tau \mu'_1$ by applying the transitive property on $=^\Gamma_\tau$:

- By (H'_1) we have that (1) $\mu_0 =^\Gamma_\tau \mu_1$.
- By Lemma ?? we have that (2) $\mu_0 =^\Gamma_\tau \mu'_0$ and (3) $\mu_1 =^\Gamma_\tau \mu'_1$.
- By (1) and (2) we have that (4) $\mu_1 =^\Gamma_\tau \mu'_0$.
- By (1) and (3) we have that (5) $\mu_0 =^\Gamma_\tau \mu'_1$.
- By (4) and (5) we conclude that (6) $\mu'_0 =^\Gamma_\tau \mu'_1$.

By applying structural induction, we have that $\text{filter}_\tau(t'_0) = \text{filter}_\tau(t'_1)$. By previous induction on c we have that $\text{filter}_\tau(t_0) = \text{filter}_\tau(t_1)$. Since $t_i \cdot t'_i$ is the concatenation of two traces t_i and t'_i , and since $\text{filter}_\tau(t_0) = \text{filter}_\tau(t_1)$ and $\text{filter}_\tau(t'_0) = \text{filter}_\tau(t'_1)$, we conclude that $\text{filter}_\tau(t_0 \cdot t'_0) = \text{filter}_\tau(t_1 \cdot t'_1)$ from which (G_2) follows.

Since (G_1) and (G_2) are satisfied, then $\text{while } e \text{ do } c'$ is NI^Γ_τ .

Subcase 3.2.3. $p \triangleq \text{if } e \text{ then } c' \text{ else } c''$.

For the typing rule *If*, we have that:

$(H_1) \Gamma \vdash e : \tau'$.

$(H_2) \Gamma \vdash c' : \tau' \text{ cmd.}$

$(H_3) \Gamma \vdash c'' : \tau' \text{ cmd.}$

For the semantics rule *Branch*, we have that:

$(H_4) \mu_i \vdash e \Rightarrow v_i$.

$(H_5) \mu_i \vdash c' \Rightarrow_{t_i} \mu'_i$.

$$(H_6) \mu_i \vdash c'' \Rightarrow_{t_i} \mu'_i.$$

Concerning c' , by induction, we conclude that:

$$(H_7) \mu'_{c'_0} =_{\tau}^{\Gamma} \mu'_{c'_1}.$$

$$(H_8) \text{filter}_{\tau}(t_0) = \text{filter}_{\tau}(t_1).$$

It follows that c' is NI_{τ}^{Γ} .

Concerning c'' , by induction, we conclude that:

$$(H_8) \mu'_{c''_0} =_{\tau}^{\Gamma} \mu'_{c''_1}.$$

$$(H_9) \text{filter}_{\tau}(t_0) = \text{filter}_{\tau}(t_1).$$

It follows that c'' is NI_{τ}^{Γ} .

Depending on τ' , we have two cases:

Subcase 3.2.4. $\Gamma \vdash e : \tau', \tau' \leq \tau$.

$$(H_{10}) \tau' \leq \tau.$$

In the case of (H_{10}) , we check if we can apply the Subtype rule on If command. We would like to check if the command If of type τ' cmd can be typable as τ' cmd, where $\tau'' \not\leq \tau'$. If the Subtype rule can be applied, the the proof of this case is analogous to Subcase 3.2.5.

Otherwise, if the Subtype rule cannot be applied, then by Lemma ??, we can conclude that:

$$(H_{11}) v_0 = v_1.$$

$$\frac{\mu_0 \vdash e \Rightarrow \text{True} \quad \mu_0 \vdash c' \Rightarrow^{t_0} \mu'_0}{\mu_0 \vdash \text{If } e \text{ then } c' \text{ else } c'' \Rightarrow^{t_0} \mu'_0}$$

$$\frac{\mu_1 \vdash e \Rightarrow \text{True} \quad \mu_1 \vdash c' \Rightarrow^{t_1} \mu'_1}{\mu_1 \vdash \text{If } e \text{ then } c' \text{ else } c'' \Rightarrow^{t_1} \mu'_1}$$

We have that $\mu'_0 =_{\tau}^{\Gamma} \mu_0$ and $\mu'_1 =_{\tau}^{\Gamma} \mu_1$. Since $\mu_0 =_{\tau}^{\Gamma} \mu_1$, we conclude that $\mu'_0 =_{\tau}^{\Gamma} \mu'_1$. Since $t_0 = t_1 = []$, then $\text{filter}_{\tau}(t_0) = \text{filter}_{\tau}(t_1)$.

$$\frac{\mu_0 \vdash e \Rightarrow \text{False} \quad \mu_0 \vdash c'' \Rightarrow^{t_0} \mu'_0}{\mu_0 \vdash \text{If } e \text{ then } c' \text{ else } c'' \Rightarrow^{t_0} \mu'_0}$$

$$\frac{\mu_1 \vdash e \Rightarrow \text{false} \quad \mu_1 \vdash c'' \Rightarrow^{t_1} \mu'_1}{\mu_1 \vdash \text{If } e \text{ then } c' \text{ else } c'' \Rightarrow^{t_1} \mu'_1}$$

We have that $\mu'_0 =_{\tau}^{\Gamma} \mu_0$ and $\mu'_1 =_{\tau}^{\Gamma} \mu_1$. Since $\mu_0 =_{\tau}^{\Gamma} \mu_1$, we conclude that $\mu'_0 =_{\tau}^{\Gamma} \mu'_1$. Since $t_0 = t_1 = []$, then $\text{filter}_{\tau}(t_0) = \text{filter}_{\tau}(t_1)$.

Subcase 3.2.5. $\Gamma \vdash e : \tau', \tau' \not\leq \tau$.

(H_{12}) $\tau' \not\leq \tau$.

By Lemma ??, we conclude that $\mu_i =_{\tau}^{\Gamma} \mu'_i$.

We prove that $\mu'_0 =_{\tau}^{\Gamma} \mu'_1$ by applying the transitive property on $=_{\tau}^{\Gamma}$.

- We have that (1) $\mu'_0 =_{\tau}^{\Gamma} \mu_0$.
- We have that (2) $\mu'_1 =_{\tau}^{\Gamma} \mu_1$.
- We have that (3) $\mu_0 =_{\tau}^{\Gamma} \mu_1$.
- By (1) and (3) we have that (4) $\mu_1 =_{\tau}^{\Gamma} \mu'_0$.
- By (2) and (3) we have that (5) $\mu_0 =_{\tau}^{\Gamma} \mu'_1$.
- By (4) and (5) we conclude that (6) $\mu'_0 =_{\tau}^{\Gamma} \mu'_1$.

Since $\text{filter}_{\tau}(t_0) = \text{filter}_{\tau}(t_1)$ and $\mu'_0 =_{\tau}^{\Gamma} \mu'_1$, then p is NI_{τ}^{Γ} .

□